Rename abses_pullback0 to abses_pullback and abses_component1_id_pullback to abses_pullback_component1_id; same for pushouts

BaerSumLaws.v
@@ -21,7 +21,7 @@ Definition  grp_compose_id_l `{Funext} {A B : Group} (f : A $-> B) : grp_homo_co
   := fun _ => idpath.
 
 Lemma abses_pushout_homotopic' `{Univalence} {A A' B : AbGroup} (f f' : A $-> A') (h : f == f')
-  : abses_pushout0 (B:=B) f $=> abses_pushout0 f'.
+  : abses_pushout (B:=B) f $=> abses_pushout f'.
 Proof.
   induction (equiv_path_grouphomomorphism h).
   apply id_transformation.
@@ -29,23 +29,23 @@ Defined.
 
 Definition abses_pushout_homotopic `{Univalence} {A A' B : AbGroup}
            (f f' : A $-> A') (h : f == f')
-  : abses_pushout0 (B:=B) f == abses_pushout0 f'
+  : abses_pushout (B:=B) f == abses_pushout f'
   := equiv_path_data_homotopy _ _ (abses_pushout_homotopic' _ _ h).
 *)
 
 (** Given a morphism [f] of short exact sequences, the pushout of the domain along [f_1] equals the pullback of the codomain along [f_3]. *)
 Lemma abses_pushout_is_pullback `{Univalence} {A A' B B' : AbGroup}
       {E : AbSES B A} {E' : AbSES B' A'} (f : AbSESMorphism E E')
-  : abses_pushout0 (component1 f) E = abses_pullback0 (component3 f) E'.
+  : abses_pushout (component1 f) E = abses_pullback (component3 f) E'.
 Proof.
   (* The morphism [f : E -> E'] factors as [E -> f_1 E -> E'], where the first map is the map defining the pushout [f_1 E] and the second map is denoted [abses_pushout_morphism_rec f] below.  This second map is the identity on the first component, so it presents its domain as the pullback of [E'] along [f_3]. *)
-  refine (abses_component1_id_pullback (abses_pushout_morphism_rec f) (fun _ => idpath)).
+  refine (abses_pullback_component1_id (abses_pushout_morphism_rec f) (fun _ => idpath)).
 Defined.
 
 (** Given a short exact sequence [A -> E -> B] and maps [f : A -> A'], [g : B' -> B], we can change the order of pushing out along [f] and pulling back along [g]. *)
 Lemma abses_reorder_pullback_pushout `{Univalence} {A A' B B' : AbGroup}
       (E : AbSES B A) (f : A $-> A') (g : B' $-> B)
-  : abses_pushout0 f (abses_pullback0 g E) = abses_pullback0 g (abses_pushout0 f E).
+  : abses_pushout f (abses_pullback g E) = abses_pullback g (abses_pushout f E).
 Proof.
   (* There are morphisms [Eg -> E] and [E -> fE] by definition of the pullback and pushout. We define [F : Eg -> fE] to be the composite. Its first and third components are [f o id] and [id o g]. *)
   pose (F := absesmorphism_compose (abses_pushout_morphism E f) (abses_pullback_morphism E g)).
@@ -128,8 +128,8 @@ Lemma baer_sum_commutative `{Univalence} {A B : AbGroup} (E F : AbSES B A)
 Proof.
   unfold abses_baer_sum.
   refine (_ @ _).
-  - refine (ap (abses_pullback0 ab_diagonal) _).
-    refine (ap (fun f => abses_pushout0 f _) ab_codiagonal_swap^ @ _).
+  - refine (ap (abses_pullback ab_diagonal) _).
+    refine (ap (fun f => abses_pushout f _) ab_codiagonal_swap^ @ _).
     refine (_^ @_).
     1: nrapply abses_pushout_compose.
     refine (ap _ (abses_pushout_is_pullback (abses_swap_morphism E F)) @ _).
@@ -154,8 +154,8 @@ Defined.
 
 (** For every [E : AbSES B A], there is an identification of the split exact sequence with the pullback of E along the zero homomorphism [B $-> B]. *)
 Definition abses_split_pullback_const `{Univalence} {A B : AbGroup} (E : AbSES B A)
-  : point (AbSES B A) = abses_pullback0 (grp_homo_const) E
-  := abses_component1_id_pullback (abses_split_morphism E) (fun _ => idpath).
+  : point (AbSES B A) = abses_pullback (grp_homo_const) E
+  := abses_pullback_component1_id (abses_split_morphism E) (fun _ => idpath).
 
 (** The identity morphism from [E] to [E]. *)
 Lemma abses_morphism_id {A B : AbGroup} (E : AbSES B A) : AbSESMorphism E E.
@@ -166,8 +166,8 @@ Defined.
 
 (** For every [E : AbSES B A], there is an identification of [E] with the pullback of [E] along [id_B]. *)
 Definition abses_id_pullback `{Univalence} {A B : AbGroup} (E : AbSES B A)
-  : E = abses_pullback0 (@grp_homo_id B) E
-  := abses_component1_id_pullback (abses_morphism_id E) (fun _ => idpath).
+  : E = abses_pullback (@grp_homo_id B) E
+  := abses_pullback_component1_id (abses_morphism_id E) (fun _ => idpath).
 
 (** Given two abelian group homomorphisms [f] and [g], their pairing [(f, g) : B -> A + A] can be written as a composite. Note that [ab_biprod_corec] is an alias for [grp_prod_corec]. *)
 Lemma ab_biprod_corec_diagonal `{Funext} {A B : AbGroup} (f g : B $-> A)
@@ -195,32 +195,32 @@ Defined.
 (** For any two [E, F : AbSES B A] and [f, g : B' $-> B], there is a morphism [Ef + Fg -> E + F] induced by the universal properties of the pullbacks of E and F, respectively. *)
 Definition abses_directsum_pullback_morphism `{Funext} {A B B' C D D' : AbGroup}
            {E : AbSES B A} {F : AbSES D C} (f : B' $-> B) (g : D' $-> D)
-  : AbSESMorphism (abses_direct_sum (abses_pullback0 f E) (abses_pullback0 g F))
+  : AbSESMorphism (abses_direct_sum (abses_pullback f E) (abses_pullback g F))
                   (abses_direct_sum E F)
   := functor_abses_directsum (abses_pullback_morphism E f) (abses_pullback_morphism F g).
 
 (** For any two [E, F : AbSES B A] and [f, g : B' $-> B], we have (E + F)(f + g) = Ef + Eg, where + denotes the direct sum. *)
 Definition abses_directsum_distributive_pullbacks `{Univalence} {A B B' : AbGroup}
            {E F : AbSES B A} (f g : B' $-> B)
-  : abses_pullback0 (functor_ab_biprod f g) (abses_direct_sum E F)
-    = abses_direct_sum (abses_pullback0 f E) (abses_pullback0 g F)
-  := (abses_component1_id_pullback (abses_directsum_pullback_morphism f g)
+  : abses_pullback (functor_ab_biprod f g) (abses_direct_sum E F)
+    = abses_direct_sum (abses_pullback f E) (abses_pullback g F)
+  := (abses_pullback_component1_id (abses_directsum_pullback_morphism f g)
         (fun _ => idpath))^.
 
 (** The analogous result follows for the Baer sum, rather than the direct sum. *)
 Lemma baer_sum_distributive_pullbacks `{Univalence} {A B B' : AbGroup}
   {E : AbSES B A} (f g : B' $-> B)
-  : abses_pullback0 (ab_homo_add f g) E = abses_baer_sum (abses_pullback0 f E) (abses_pullback0 g E).
+  : abses_pullback (ab_homo_add f g) E = abses_baer_sum (abses_pullback f E) (abses_pullback g E).
 Proof.
   unfold abses_baer_sum, ab_homo_add.
   refine ((abses_pullback_compose (B1:=ab_biprod B B) _ _ E)^ @ _).
-  refine (ap (abses_pullback0 _) (abses_pushout_is_pullback (abses_codiagonal E))^ @ _).
+  refine (ap (abses_pullback _) (abses_pushout_is_pullback (abses_codiagonal E))^ @ _).
   unfold abses_codiagonal, component1.
   refine ((abses_reorder_pullback_pushout _ _ _)^ @ _ @ abses_reorder_pullback_pushout _ _ _).
-  refine (ap (abses_pushout0 _) _).
-  refine (ap (fun h => abses_pullback0 h _) (ab_biprod_corec_diagonal _ _) @ _).
+  refine (ap (abses_pushout _) _).
+  refine (ap (fun h => abses_pullback h _) (ab_biprod_corec_diagonal _ _) @ _).
   refine ((abses_pullback_compose _ _ (abses_direct_sum E E))^ @ _).
-  exact (ap (abses_pullback0 _) (abses_directsum_distributive_pullbacks f g)).
+  exact (ap (abses_pullback _) (abses_directsum_distributive_pullbacks f g)).
 Defined.
 
 (** Adding the zero homomorphism to any other [f : A $-> A] has no effect. *)
@@ -242,9 +242,9 @@ Lemma baer_sum_unit_r `{Univalence} {A B : AbGroup} (E : AbSES B A)
 Proof.
   refine (ap (abses_baer_sum E) _ @ _).
   - exact (abses_split_pullback_const E).
-  - refine (ap (fun F => abses_baer_sum F (abses_pullback0 grp_homo_const E)) (abses_id_pullback E) @ _).
+  - refine (ap (fun F => abses_baer_sum F (abses_pullback grp_homo_const E)) (abses_id_pullback E) @ _).
     refine ((baer_sum_distributive_pullbacks grp_homo_id grp_homo_const)^ @ _).
-    refine (ap (fun f => abses_pullback0 f E) (ab_homo_add_zero_r _) @ _).
+    refine (ap (fun f => abses_pullback f E) (ab_homo_add_zero_r _) @ _).
     symmetry; apply abses_id_pullback.
 Defined.
 
@@ -271,21 +271,21 @@ Defined.
 
 (** We can now prove the inverse laws for the Baer sum, which state that for any [E : AbSES B A], the pullback of [E] along [-id_B] acts as an additive inverse for [E] with respect to the Baer sum. *)
 Lemma baer_sum_inverse_l `{Univalence} {A B : AbGroup} (E : AbSES B A)
-  : abses_baer_sum E (abses_pullback0 (-grp_homo_id) E) = point (AbSES B A).
+  : abses_baer_sum E (abses_pullback (-grp_homo_id) E) = point (AbSES B A).
 Proof.
-  refine (ap (fun F => abses_baer_sum F (abses_pullback0 _ E)) (abses_id_pullback E) @ _).
+  refine (ap (fun F => abses_baer_sum F (abses_pullback _ E)) (abses_id_pullback E) @ _).
   refine ((baer_sum_distributive_pullbacks grp_homo_id (-grp_homo_id))^ @ _).
-  refine (ap (fun f => abses_pullback0 f _) (ab_negate_homo_cancel _) @ _).
+  refine (ap (fun f => abses_pullback f _) (ab_negate_homo_cancel _) @ _).
   symmetry; apply abses_split_pullback_const.
 Defined.
 
 (** The right inverse law follows by commutativity. *)
 Definition baer_sum_inverse_r `{Univalence} {A B : AbGroup} (E : AbSES B A)
-  : abses_baer_sum (abses_pullback0 (-grp_homo_id) E) E = point (AbSES B A)
+  : abses_baer_sum (abses_pullback (-grp_homo_id) E) E = point (AbSES B A)
   := baer_sum_commutative _ _ @ baer_sum_inverse_l _.
 
 (** Given [E : AbSES B A'] and [F : AbSES B A] and a morphism [f : E -> F], the pushout of [E] along [f_1] is [F] if [f_3] is homotopic to [id_B]. *)
-Lemma abses_component3_id_pushout' `{Univalence}
+Lemma abses_pushout_component3_id' `{Univalence}
       {A A' B : AbGroup} {E : AbSES B A'} {F : AbSES B A}
       (f : AbSESMorphism E F) (h : component3 f == grp_homo_id)
   : abses_pushout (component1 f) E $== F.
@@ -300,11 +300,11 @@ Proof.
 Defined.
 
 (** A version with equality instead of path data. *)
-Definition abses_component3_id_pushout `{Univalence}
+Definition abses_pushout_component3_id `{Univalence}
            {A A' B : AbGroup} {E : AbSES B A'} {F : AbSES B A}
            (f : AbSESMorphism E F) (h : component3 f == grp_homo_id)
   : abses_pushout (component1 f) E = F
-  := equiv_path_abses_iso (abses_component3_id_pushout' f h).
+  := equiv_path_abses_iso (abses_pushout_component3_id' f h).
 
 (** Given short exact sequences [E] and [F] and homomorphisms [f : A' $-> A] and [g : D' $-> D], there is a morphism [E + F -> fE + gF] induced by the universal properties of the pushouts of [E] and [F]. *)
 Definition abses_directsum_pushout_morphism `{Univalence}
@@ -318,7 +318,7 @@ Definition abses_directsum_distributive_pushouts `{Univalence}
            {A A' B : AbGroup} {E F : AbSES B A'} (f g : A' $-> A)
   : abses_pushout (functor_ab_biprod f g) (abses_direct_sum E F)
     = abses_direct_sum (abses_pushout f E) (abses_pushout g F)
-  := abses_component3_id_pushout (abses_directsum_pushout_morphism f g) (fun _ => idpath).
+  := abses_pushout_component3_id (abses_directsum_pushout_morphism f g) (fun _ => idpath).
 
 (** The analogous result for the Baer sum. *)
 Lemma baer_sum_distributive_pushouts `{Univalence}
@@ -333,7 +333,7 @@ Proof.
   refine ((abses_pushout_compose _ _ E)^ @ _).
   refine (ap (abses_pushout _) (abses_pushout_is_pullback (abses_diagonal E)) @ _).
   refine (abses_reorder_pullback_pushout _ _ _ @ _).
-  exact (ap (abses_pullback0 _) (abses_directsum_distributive_pushouts f g)).
+  exact (ap (abses_pullback _) (abses_directsum_distributive_pushouts f g)).
 Defined.
 
 (*
